Making digraph work with generic nodes.

CircuitPath.dfy
@@ -1,28 +1,11 @@
-include "../libraries/src/Wrappers.dfy"
-include "SeqNatToNat.dfy"
-include "circuit.dfy"
-
 module CircuitPath {
 
-    import opened Wrappers
+    import opened Std.Wrappers
+    import Seq = Std.Collections.Seq
+    import SeqNatToNat
+    import SeqExt
     import opened Circuit
-
-    datatype Path = PathNil | PathCons(head: HPNP, tail: Path)
-
-    function PathLength(p: Path): nat
-    {
-        match p
-        case PathNil => 0
-        case PathCons(head, tail) => 1 + PathLength(tail)
-    }
-
-    function PathStart(p: Path): HPNP
-        requires p.PathCons?
-    {
-        match p
-        case PathCons(head, Nil) => head
-        case PathCons(head, tail) => PathStart(tail)
-    }
+    import DG
 
     predicate {:opaque} HPNPOtoIConnected(c: Circuit, a: HPNP, b: HPNP)
         requires CircuitValid(c)
@@ -37,7 +20,7 @@ module CircuitPath {
             match a_nk
             case CInput => (
                 match a.hpn.hp
-                // This is a top level input. It's not connected to anything.
+                // This is an output from a CInput. It's not connected.
                 case Top => false
                 case Level(hier_n, parent_hp) =>
                     // If it's an input inside a hier node, then it connects to
@@ -67,8 +50,14 @@ module CircuitPath {
     }
 
     predicate {:opaque} HPNPItoOConnected(c: Circuit, a: HPNP, b: HPNP)
+        requires CircuitValid(c)
+        requires HPNPValidInput(c, a)
+        requires HPNPValidOutput(c, b)
     {
-        false
+        var a_c := HierarchyPathCircuit(c, a.hpn.hp);
+        var inp := NP(a.hpn.n, a.p);
+        var onp := NP(b.hpn.n, b.p);
+        c.PortSource(inp) == Some(onp)
     }
 
     predicate {:opaque} HPNPConnected(c: Circuit,  a: HPNP, b: HPNP)
@@ -80,210 +69,98 @@ module CircuitPath {
             HPNPOtoIConnected(c, a, b))
     }
 
-    predicate PathValid(c: Circuit, p: Path)
+    function HierarchyPathToNatInternal(hp: HierarchyPath, hn: nat) : (r: nat)
+    {
+        match hp
+        case Top => hn
+        case Level(n, parent) =>
+            var new_hn := SeqNatToNat.NatsToNat([n as nat, hn]) as nat;
+            HierarchyPathToNatInternal(parent, new_hn)
+    }
+
+    function HPNodeToNat(hpn: HPNode) : (r: nat)
+    {
+        HierarchyPathToNatInternal(hpn.hp, hpn.n as nat)
+    }
+
+    function HPNPToNat(hpnp: HPNP) : (r: nat)
+    {
+        SeqNatToNat.NatsToNat([HPNodeToNat(hpnp.hpn) as nat, hpnp.p as nat])
+    }
+
+    lemma NatsToNatUnique(a: nat, b: nat, c: nat, d: nat)
+        requires (a, b) != (c, d)
+        ensures SeqNatToNat.NatsToNat([a, b]) != SeqNatToNat.NatsToNat([c, d])
+    {
+    }
+
+    lemma NatsToNatBounded(a: nat, b: nat, c: nat, d: nat)
+        requires (a < c) && (b < d)
+        ensures SeqNatToNat.NatsToNat([a, b]) < SeqNatToNat.NatsToNat([c, d])
+    {
+    }
+
+    function HPNPBound(c: Circuit): nat
+    {
+        0
+    }
+
+    function CtoG(c: Circuit): (g: DG.Digraph<HPNP>)
         requires CircuitValid(c)
-        decreases p
     {
-        match p
-        case PathNil => true
-        case PathCons(head, PathCons(head2, tail)) =>
-            HPNPValid(c, head) && HPNPConnected(c, head2, head) &&
-            PathValid(c, PathCons(head2, tail))
-        case PathCons(head, tail) =>
-            HPNPValid(c, head) && PathValid(c, tail)
+        DG.Digraph(
+            hpnp => HPNPValid(c, hpnp),
+            (a, b) => HPNPConnected(c, a, b),
+            HPNPToNat,
+            HPNPBound(c)
+        )
     }
 
-    predicate ReversePathValid(c: Circuit, p: Path)
+    lemma HPNPBounded(c: Circuit, hpnp: HPNP)
         requires CircuitValid(c)
-        decreases p
+        requires HPNPToNat(hpnp) >= HPNPBound(c)
+        ensures !HPNPValid(c, hpnp)
     {
-        match p
-        case PathNil => true
-        case PathCons(head, PathCons(head2, tail)) =>
-            HPNPValid(c, head) && HPNPConnected(c, head, head2) &&
-            ReversePathValid(c, PathCons(head2, tail))
-        case PathCons(head, tail) =>
-            HPNPValid(c, head) && ReversePathValid(c, tail)
     }
 
-    predicate {:opaque} PathExcludes(p: Path, exclusion: set<HPNP>)
-    {
-        match p
-        case Nil => true
-        case PathCons(head, tail) => head !in exclusion && PathExcludes(tail, exclusion)
-    }
-
-    predicate {:opaque} PathContainsNP(p: Path, np: HPNP)
-    {
-        match p
-        case Nil => false
-        case PathCons(head, tail) => head == np || PathContainsNP(tail, np)
-    }
-
-    lemma NPInExclusionNotInPath(p: Path, exclusion: set<HPNP>, np: HPNP)
-        requires PathExcludes(p, exclusion)
-        requires np in exclusion
-        ensures !PathContainsNP(p, np)
-    {
-        reveal PathExcludes();
-        reveal PathContainsNP();
-    }
-
-    predicate NextNode(c: Circuit, n: HPNP, m: HPNP)
+    lemma NoSelfConnections(c: Circuit, n: HPNP)
         requires CircuitValid(c)
-        requires HPNPValid(c, n)
+        ensures !HPNPConnected(c, n, n)
     {
-        HPNPConnected(c, n, m)
     }
 
-    function PathAppend(p: Path, n: HPNP): (r: Path)
-    {
-        PathCons(n, p)
-    }
-
-    lemma PathAppendValid(c: Circuit, p: Path, n: HPNP)
-        // Add a node onto a path.
+    lemma ConnectedNodesValid(c: Circuit, n: HPNP, m: HPNP)
         requires CircuitValid(c)
-        requires HPNPValid(c, n)
-        requires p.PathCons?
-        requires HPNPConnected(c, p.head, n)
-        requires PathValid(c, p)
-        ensures
-            var r := PathAppend(p, n);
-            PathValid(c, r)
+        ensures HPNPConnected(c, n, m) ==> HPNPValid(c, n) && HPNPValid(c, m)
     {
     }
 
-    lemma ReversePathAppendValid(c: Circuit, p: Path, n: HPNP)
-        // Add a node onto a path.
+    lemma HPNPNatsUnique(a: HPNP, b: HPNP)
+        ensures (a != b) ==> HPNPToNat(a) != HPNPToNat(b)
+    {
+    }
+
+    lemma CtoGValid(c: Circuit)
         requires CircuitValid(c)
-        requires HPNPValid(c, n)
-        requires p.PathCons?
-        requires HPNPConnected(c, n, p.head)
-        requires ReversePathValid(c, p)
-        ensures
-            var r := PathAppend(p, n);
-            ReversePathValid(c, r)
+        ensures DG.DigraphValid(CtoG(c))
     {
-    }
-
-    function ReversePathInternal(p: Path, partial_reversed: Path): (r: Path)
-        ensures PathLength(r) == PathLength(p) + PathLength(partial_reversed)
-    {
-        match p
-        case PathNil => partial_reversed
-        case PathCons(head, tail) => ReversePathInternal(tail, PathCons(head, partial_reversed))
-    }
-
-    lemma ReversedLengthOnePathIsUnchanged(p: Path)
-        requires p.PathCons?
-        requires p.tail == PathNil
-        ensures ReversePath(p) == p
-    {
-        var head := p.head;
-        assert p == PathCons(head, PathNil);
-        assert ReversePath(p) == ReversePathInternal(p, PathNil);
-    }
-
-    lemma ReversePathInternalForwardValid(c: Circuit, p: Path, partial_reversed: Path)
-        requires CircuitValid(c)
-        requires PathValid(c, p)
-        requires ReversePathValid(c, partial_reversed)
-        requires (p.PathCons? && partial_reversed.PathCons?) ==> HPNPConnected(c, p.head, partial_reversed.head)
-        ensures
-            var r := ReversePathInternal(p, partial_reversed);
-            ReversePathValid(c, r)
-    {
-        match p
-        case PathNil => {}
-        case PathCons(head, tail) =>
-            ReversePathInternalForwardValid(c, tail, PathCons(head, partial_reversed));
-    }
-
-    lemma ReversePathForwardValid(c: Circuit, p: Path)
-        requires CircuitValid(c)
-        requires PathValid(c, p)
-        ensures
-            var r := ReversePath(p);
-            ReversePathValid(c, r)
-    {
-        ReversePathInternalForwardValid(c, p, PathNil);
-    }
-
-    lemma ReversePathInternalBackwardValid(c: Circuit, p: Path, partial_reversed: Path)
-        requires CircuitValid(c)
-        requires ReversePathValid(c, p)
-        requires PathValid(c, partial_reversed)
-        requires (p.PathCons? && partial_reversed.PathCons?) ==> HPNPConnected(c, partial_reversed.head, p.head)
-        ensures
-            var r := ReversePathInternal(p, partial_reversed);
-            PathValid(c, r)
-    {
-        match p
-        case PathNil => {}
-        case PathCons(head, tail) =>
-            ReversePathInternalBackwardValid(c, tail, PathCons(head, partial_reversed));
-    }
-
-    lemma ReversePathBackwardValid(c: Circuit, p: Path)
-        requires CircuitValid(c)
-        requires ReversePathValid(c, p)
-        ensures
-            var r := ReversePath(p);
-            PathValid(c, r)
-    {
-        ReversePathInternalBackwardValid(c, p, PathNil);
-    }
-
-    function ReversePath(p: Path): (r: Path)
-        ensures PathLength(p) == PathLength(r)
-    {
-        ReversePathInternal(p, PathNil)
-    }
-    
-    function PathPrepend(p: Path, n: HPNP): (r: Path)
-    {
-        var reversed := ReversePath(p);
-        var appended := PathAppend(reversed, n);
-        var prepended := ReversePath(appended);
-        prepended
-    }
-
-    lemma PathStartIsReversedHead(p: Path)
-        requires p.PathCons?
-        ensures ReversePath(p).head == PathStart(p)
-    {
-        match p
-        case PathCons(head, PathNil) => {
-            assert head == PathStart(p);
-            assert ReversePath(p) == ReversePathInternal(p, PathNil);
-            assert ReversePath(p).head == head;
+        var g := CtoG(c);
+        forall n: HPNP, m: HPNP
+            ensures HPNPToNat(n) >= HPNPBound(c) ==> !HPNPValid(c, n)
+            ensures !HPNPConnected(c, n, n)
+            ensures HPNPConnected(c, n, m) ==> HPNPValid(c, n) && HPNPValid(c, m)
+            ensures (n != m) ==> HPNPToNat(n) != HPNPToNat(m)
+        {
+            HPNPBounded(c, n);
+            NoSelfConnections(c, n);
+            ConnectedNodesValid(c, n, m);
+            HPNPNatsUnique(n, m);
         }
-        case PathCons(head, tail) => {
-            PathStartIsReversedHead(tail);
-            assert ReversePath(tail).head == PathStart(tail);
-        }
-    }
-
-    lemma PathPrependValid(c: Circuit, p: Path, n: HPNP)
-        // Add a node onto a path.
-        requires CircuitValid(c)
-        requires HPNPValid(c, n)
-        requires p.PathCons?
-        requires HPNPConnected(c, PathStart(p), n)
-        requires PathValid(c, p)
-        ensures
-            var r := PathPrepend(p, n);
-            PathValid(c, r);
-    {
-        var reversed := ReversePath(p);
-        assert reversed.head == PathStart(p);
-        ReversePathForwardValid(c, p);
-        assert ReversePathValid(c, reversed);
-        var appended := PathAppend(reversed, n);
-        ReversePathAppendValid(c, reversed, n);
-        assert ReversePathValid(c, appended);
-        var prepended := ReversePath(appended);
+        assert (forall n: HPNP :: HPNPToNat(n) >= HPNPBound(c) ==> !HPNPValid(c, n));
+        assert (forall n: HPNP :: !HPNPConnected(c, n, n));
+        assert (forall n: HPNP, m: HPNP :: HPNPConnected(c, n, m) ==> HPNPValid(c, n) && HPNPValid(c, m));
+        assert (forall n: HPNP, m: HPNP :: n != m ==> HPNPToNat(n) != HPNPToNat(m));
+        reveal DG.DigraphValid();
     }
 
 }
